theories/rules/rules_EStoreId.v
@@ -19,13 +19,13 @@ Section cap_lang_rules.
   Implicit Types lmem : LMem.
 
   (* TODO @Denis *)
-  Lemma wp_estoreid E pc_p pc_b pc_e pc_a pc_v pca_v lw r1 r2 r3 :
+  Lemma wp_estoreid E pc_p pc_b pc_e pc_a pc_v lw r1 r2 r3 :
     decodeInstrWL lw = EStoreId r1 r2 r3 →
     isCorrectLPC (LCap pc_p pc_b pc_e pc_a pc_v) →
 
-    {{{ PC ↦ᵣ LCap pc_p pc_b pc_e pc_a pc_v ∗ (pc_a, pca_v) ↦ₐ lw }}}
+    {{{ PC ↦ᵣ LCap pc_p pc_b pc_e pc_a pc_v ∗ (pc_a, pc_v) ↦ₐ lw }}}
       Instr Executable @ E
-    {{{ RET FailedV; PC ↦ᵣ LCap pc_p pc_b pc_e pc_a pc_v ∗ (pc_a, pca_v) ↦ₐ lw }}}.
+    {{{ RET FailedV; PC ↦ᵣ LCap pc_p pc_b pc_e pc_a pc_v ∗ (pc_a, pc_v) ↦ₐ lw }}}.
   Proof.
     iIntros (Hinstr Hvpc φ) "[Hpc Hpca] Hφ".
     apply isCorrectLPC_isCorrectPC_iff in Hvpc; cbn in Hvpc.
@@ -40,8 +40,8 @@ Section cap_lang_rules.
     apply prim_step_exec_inv in Hstep as (-> & -> & (c & -> & Hstep)).
     iNext; iIntros "_".
     iSplitR; auto. eapply step_exec_inv in Hstep; eauto.
-    2: eapply state_phys_log_reg_get_word in H2; eauto.
-    2: eapply state_phys_log_mem_get_word in H3; eauto.
+    2: eapply state_phys_corresponds_reg ; eauto ; cbn ; eauto.
+    2: eapply state_phys_corresponds_mem_PC ; eauto; cbn ; eauto.
     cbn in Hstep; simplify_eq.
     iModIntro.
     iSplitR "Hφ Hpc Hpca"; last (iApply "Hφ" ; iFrame).
